steel/Zeta.Steel.HashValue.fst
@@ -1,0 +1,104 @@
+module Zeta.Steel.HashValue
+open Steel.ST.Util
+open Zeta.Steel.Util
+module P = Zeta.Steel.Parser
+module T = Zeta.Steel.FormatsManual
+module Blake = Hacl.Blake2b_32
+module A = Steel.ST.Array
+module U8 = FStar.UInt8
+
+assume
+val spec_parser_value: P.spec_parser T.value
+
+assume
+val spec_serializer_value: P.spec_serializer spec_parser_value
+
+assume
+val serialize_value : P.serializer spec_serializer_value
+
+/// This is an ad hoc bound due to a bound on Blake hashable inputs
+assume
+val serialized_value_length (s:T.value)
+  : Lemma  (Seq.length (spec_serializer_value s) <= 4096)
+           [SMTPat (Seq.length (spec_serializer_value s))]
+
+let bytes_as_u256 (b:Seq.seq U8.t { Seq.length b == 32 })
+  : GTot T.u256
+  = let u64s = FStar.Endianness.seq_uint64_of_le 4 b in
+    { v0 = Seq.index u64s 0;
+      v1 = Seq.index u64s 1;
+      v2 = Seq.index u64s 2;
+      v3 = Seq.index u64s 3 }
+
+let hashfn (v:T.value)
+  : GTot T.hash_value
+  = let bytes = spec_serializer_value v in
+    let hash_bytes = Blake.spec bytes 0 Seq.empty 32 in
+    bytes_as_u256 hash_bytes
+
+noeq
+type hasher_t = {
+  serialization_buffer: A.larray U8.t 4096;
+  hash_buffer: A.larray U8.t 32
+}
+
+[@@__steel_reduce__; __reduce__]
+let inv (h:hasher_t) =
+  exists_ (array_pts_to h.hash_buffer) `star`
+  exists_ (array_pts_to h.serialization_buffer)
+
+let alloc (_:unit)
+  : STT hasher_t emp inv
+  = let hb = A.alloc 0uy 32ul in
+    intro_exists _ (array_pts_to hb);
+    let sb = A.alloc 0uy 4096ul in
+    intro_exists _ (array_pts_to sb);
+    let res = {
+      serialization_buffer = sb;
+      hash_buffer = hb
+    } in
+    rewrite (exists_ (array_pts_to sb))
+            (exists_ (array_pts_to res.serialization_buffer));
+    rewrite (exists_ (array_pts_to hb))
+            (exists_ (array_pts_to res.hash_buffer));
+    return res
+
+let array_free (a:A.array 'a)
+  : STT unit (exists_ (array_pts_to a)) (fun _ -> emp)
+  = let v = elim_exists () in
+    intro_exists_erased v (A.pts_to a full_perm);
+    A.free a
+
+let free (h:hasher_t)
+  : STT unit (inv h) (fun _ -> emp)
+  = array_free h.hash_buffer;
+    array_free h.serialization_buffer
+
+let read_hash_u256 (#hv:Ghost.erased _)
+                   (hb:A.larray U8.t 32)
+  : ST T.u256
+    (A.pts_to hb full_perm hv)
+    (fun _ -> A.pts_to hb full_perm hv)
+    (requires True)
+    (ensures fun res ->
+      Seq.length hv == 32 /\
+      res == bytes_as_u256 hv)
+  = admit__()
+
+let hash_value (h:hasher_t)
+               (v:T.value)
+  : ST T.hash_value
+    (inv h)
+    (fun _ -> inv h)
+    (requires True)
+    (ensures fun res -> hashfn v == res)
+  = let n = serialize_value 4096ul 0ul h.serialization_buffer v in
+    let hv = elim_exists  #_ #_ #(array_pts_to h.hash_buffer) () in
+    let sv = elim_exists () in
+    elim_pure _;
+    A.pts_to_length h.hash_buffer _;
+    Blake.blake2b 32ul h.hash_buffer n h.serialization_buffer;
+    let res = read_hash_u256 h.hash_buffer in
+    intro_exists _ (array_pts_to h.serialization_buffer);
+    intro_exists _ (array_pts_to h.hash_buffer);
+    return res
