steel/Zeta.Steel.VerifierTypes.fst
@@ -41,7 +41,8 @@ type thread_state_t = {
   last_verified_epoch: R.ref (option M.epoch_id);
   processed_entries: G.ref (Seq.seq log_entry);
   app_results  : G.ref M.app_results;
-  serialization_buffer: A.larray U8.t 4096
+  serialization_buffer: A.larray U8.t 4096;
+  hasher       : HashValue.hasher_t
 }
 
 let thread_id t = t.thread_id
@@ -57,7 +58,8 @@ let thread_state_inv_core (t:thread_state_t)
     R.pts_to t.last_verified_epoch full tsm.last_verified_epoch `star`
     G.pts_to t.processed_entries full tsm.processed_entries `star`
     G.pts_to t.app_results full tsm.app_results `star`
-    exists_ (array_pts_to t.serialization_buffer)
+    exists_ (array_pts_to t.serialization_buffer) `star`
+    HashValue.inv t.hasher
 
 let intro_thread_state_inv_core #o
                            (tsm:M.thread_state_model)
@@ -77,7 +79,8 @@ let intro_thread_state_inv_core #o
       R.pts_to t.last_verified_epoch full lve `star`
       G.pts_to t.processed_entries full pe `star`
       G.pts_to t.app_results full ar `star`
-      exists_ (array_pts_to t.serialization_buffer))
+      exists_ (array_pts_to t.serialization_buffer) `star`
+      HashValue.inv t.hasher)
      (fun _ -> thread_state_inv_core t tsm)
      (requires
        tsm.failed == f /\
@@ -96,7 +99,8 @@ let intro_thread_state_inv_core #o
               R.pts_to t.last_verified_epoch _ _ `star`
               G.pts_to t.processed_entries _ _ `star`
               G.pts_to t.app_results _ _ `star`
-              exists_ (array_pts_to t.serialization_buffer))
+              exists_ (array_pts_to t.serialization_buffer) `star`
+              HashValue.inv t.hasher)
              (thread_state_inv_core t tsm)
 
 [@@__reduce__]
